stop using bool | xreal for ehoare

src/ecCallbyValue.ml
@@ -496,22 +496,18 @@ and cbv (st : state) (s : subst) (f : form) (args : args) : form =
     assert (Args.isempty args);
     assert (not (Subst.has_mem s mhr));
     let ehf_pr  = norm st s hf.ehf_pr  in
-    let ehf_epr = norm st s hf.ehf_epr in
     let ehf_po  = norm st s hf.ehf_po  in
-    let ehf_epo = norm st s hf.ehf_epo in
     let ehf_f   = norm_xfun st s hf.ehf_f in
-    f_eHoareF_r { ehf_pr; ehf_epr; ehf_f; ehf_po; ehf_epo }
+    f_eHoareF_r { ehf_pr; ehf_f; ehf_po; }
 
   | FeHoareS hs ->
     assert (Args.isempty args);
     assert (not (Subst.has_mem s (fst hs.ehs_m)));
     let ehs_pr  = norm st s hs.ehs_pr in
-    let ehs_epr = norm st s hs.ehs_epr in
     let ehs_po  = norm st s hs.ehs_po in
-    let ehs_epo = norm st s hs.ehs_epo in
     let ehs_s   = norm_stmt s hs.ehs_s in
     let ehs_m   = norm_me s hs.ehs_m in
-    f_eHoareS_r { ehs_pr; ehs_epr; ehs_po; ehs_epo; ehs_s; ehs_m }
+    f_eHoareS_r { ehs_pr; ehs_po; ehs_s; ehs_m }
 
   | FcHoareF chf ->
     assert (Args.isempty args);
