src/ecPV.ml
@@ -350,10 +350,10 @@ module PV = struct
           in_mem_scope env fv [fst hs.hs_m] [hs.hs_pr; hs.hs_po]
 
       | FeHoareF hf ->
-          in_mem_scope env fv [mhr] [hf.ehf_pr; hf.ehf_epr; hf.ehf_po; hf.ehf_epo]
+          in_mem_scope env fv [mhr] [hf.ehf_pr; hf.ehf_po]
 
       | FeHoareS hs ->
-          in_mem_scope env fv [fst hs.ehs_m] [hs.ehs_pr; hs.ehs_epr; hs.ehs_po; hs.ehs_epo]
+          in_mem_scope env fv [fst hs.ehs_m] [hs.ehs_pr; hs.ehs_po]
 
       | FcHoareF chf ->
           let fv = in_mem_scope env fv [mhr] [chf.chf_pr; chf.chf_po] in
