src/ecParser.mly
@@ -1361,9 +1361,9 @@ hoare_body(P):
     { PFhoareF (pre, mp, post) }
 
 ehoare_body(P):
-  mp=loc(fident) COLON pre=form_r(P) PIPE epre=form_r(P) LONGARROW
-                       post=form_r(P) PIPE epost=form_r(P)
-    { PFehoareF (pre, epre, mp, post, epost) }
+  mp=loc(fident) COLON pre=form_r(P) LONGARROW
+                       post=form_r(P)
+    { PFehoareF (pre, mp, post) }
 
 phoare_body(P):
   LBRACKET mp=loc(fident) COLON
@@ -2669,19 +2669,15 @@ cbv:
 | CBV l=qoident+ { `Delta l  :: simplify_red  }
 | CBV DELTA      { `Delta [] :: simplify_red }
 
-eform:
-| p=form             { Single p     }
-| p=form PIPE f=form { Double(p, f) }
-
 conseq:
 | empty                            { None, None }
 | UNDERSCORE LONGARROW UNDERSCORE  { None, None }
-| f1=eform LONGARROW               { Some f1, None }
-| f1=eform LONGARROW UNDERSCORE    { Some f1, None }
-| f2=eform                         { None, Some f2 }
-| LONGARROW f2=eform               { None, Some f2 }
-| UNDERSCORE LONGARROW f2=eform    { None, Some f2 }
-| f1=eform LONGARROW f2=eform      { Some f1, Some f2 }
+| f1=form LONGARROW               { Some f1, None }
+| f1=form LONGARROW UNDERSCORE    { Some f1, None }
+| f2=form                         { None, Some f2 }
+| LONGARROW f2=form               { None, Some f2 }
+| UNDERSCORE LONGARROW f2=form    { None, Some f2 }
+| f1=form LONGARROW f2=form       { Some f1, Some f2 }
 
 conseq_xt:
 | c=conseq                                     { c, None }
@@ -2770,17 +2766,17 @@ semrndpos:
     { Double (n1, n2) }
 
 while_tac_info:
-| inv=form_or_double_form
+| inv=sform
     { { wh_inv = inv; wh_vrnt = None; wh_bds = None; } }
 
 | inv=sform vrnt=sform
-    { { wh_inv = Single inv; wh_vrnt = Some vrnt; wh_bds = None; } }
+    { { wh_inv = inv; wh_vrnt = Some vrnt; wh_bds = None; } }
 
 | inv=sform vrnt=sform k=sform eps=sform
-    { { wh_inv = Single inv; wh_vrnt = Some vrnt; wh_bds = Some (`Bd (k, eps)); } }
+    { { wh_inv = inv; wh_vrnt = Some vrnt; wh_bds = Some (`Bd (k, eps)); } }
 
 | inv=sform vrnt=sform k=sform TIME co=costs(none)
-    { { wh_inv = Single inv; wh_vrnt = Some vrnt; wh_bds = Some (`Cost (k, co)); } }
+    { { wh_inv = inv; wh_vrnt = Some vrnt; wh_bds = Some (`Cost (k, co)); } }
 
 async_while_tac_info:
 | LBRACKET t1=expr COMMA f1=form RBRACKET
@@ -3042,9 +3038,6 @@ form_or_double_form:
 | LPAREN UNDERSCORE? COLON f1=form LONGARROW f2=form RPAREN
     { Double (f1, f2) }
 
-| LPAREN  f1=form PIPE f2=form RPAREN
-    { Double (f1, f2) }
-
 %inline if_cost_option:
 | CEQ f=sform    {f}
 
@@ -3109,9 +3102,6 @@ phltactic:
 
 | PROC bad=sform p=sform q=sform?
    { Pfun (`Upto (bad, p, q)) }
-
-| PROC LPAREN inv=form PIPE einv=form RPAREN
-   { Pfun (`Ehoare (inv, einv)) }
 
 | PROC STAR
    { Pfun `Code }
