src/ecTyping.ml
@@ -3605,18 +3605,14 @@ and trans_form_or_pattern
           unify_or_fail penv ue pre.pl_loc  ~expct:tbool pre' .f_ty;
           unify_or_fail qenv ue post.pl_loc ~expct:tbool post'.f_ty;
           f_hoareF pre' fpath post'
-    | PFehoareF (pre, epre, gp, post, epost) ->
+    | PFehoareF (pre, gp, post) ->
         let fpath = trans_gamepath env gp in
         let penv, qenv = EcEnv.Fun.hoareF fpath env in
         let pre'  = transf penv pre in
-        let epre'  = transf penv epre in
         let post' = transf qenv post in
-        let epost' = transf qenv epost in
-          unify_or_fail penv ue pre.pl_loc  ~expct:tbool   pre' .f_ty;
-          unify_or_fail penv ue pre.pl_loc  ~expct:txreal epre'.f_ty;
-          unify_or_fail qenv ue post.pl_loc ~expct:tbool   post'.f_ty;
-          unify_or_fail qenv ue post.pl_loc ~expct:txreal epost'.f_ty;
-          f_eHoareF pre' epre' fpath post' epost'
+          unify_or_fail penv ue pre.pl_loc  ~expct:txreal pre'.f_ty;
+          unify_or_fail qenv ue post.pl_loc ~expct:txreal post'.f_ty;
+          f_eHoareF pre' fpath post'
 
     | PFBDhoareF (pre, gp, post, hcmp, bd) ->
         let fpath = trans_gamepath env gp in
