src/phl/ecPhlConseq.mli
@@ -23,8 +23,8 @@ val t_cHoareF_conseq_c    : cost -> FApi.backward
 val t_cHoareS_conseq_c    : cost -> FApi.backward
 val t_cHoareF_conseq_full : form -> form -> cost -> FApi.backward
 val t_cHoareS_conseq_full : form -> form -> cost -> FApi.backward
-val t_ehoareF_conseq      : form -> form -> form -> form -> FApi.backward
-val t_ehoareS_conseq      : form -> form -> form -> form -> FApi.backward
+val t_ehoareF_conseq      : form -> form -> FApi.backward
+val t_ehoareS_conseq      : form -> form -> FApi.backward
 val t_bdHoareS_conseq_bd  : hoarecmp -> form -> FApi.backward
 val t_bdHoareF_conseq_bd  : hoarecmp -> form -> FApi.backward
 
@@ -42,7 +42,7 @@ val t_bdHoareS_conseq_nm  : form -> form -> FApi.backward
 val t_equivS_conseq_bd : side -> EcFol.form -> EcFol.form ->FApi.backward
 
 (* -------------------------------------------------------------------- *)
-val t_conseq : ?epre:form -> ?epost:form -> form -> form -> FApi.backward
+val t_conseq : form -> form -> FApi.backward
 
 (* -------------------------------------------------------------------- *)
 val process_conseq   : bool -> conseq_ppterm option tuple3 -> FApi.backward
