src/phl/ecPhlWp.ml
@@ -100,7 +100,7 @@ module LowInternal = struct
         wp_asgn_aux None memenv lv e letspf
 
       | Srnd(lv, distr) ->
-        let (lets,(p,f)) = letspf in
+        let (lets,f) = letspf in
         let ty_distr = proj_distr_ty env (EcTypes.e_ty distr) in
         let x_id = EcIdent.create (symbol_of_lv lv) in
         let x = f_local x_id ty_distr in
@@ -108,25 +108,20 @@ module LowInternal = struct
         let distr = EcFol.form_of_expr m distr in
         let let1 = lv_subst ?c_pre:None m lv x in
         let lets = let1 :: lets in
-        let p = mk_let_of_lv_substs env (lets,p) in
         let f = mk_let_of_lv_substs env (lets,f) in
-        let p = f_forall [(x_id,GTty ty_distr)] (f_imp (f_in_supp x distr) p) in
         let f = f_Ep ty_distr distr (f_lambda [(x_id,GTty ty_distr)] f) in
-        ([], (p, f))
+        ([], f)
 
       | Sif(e, s1, s2) ->
-        let r1,(lets1,(p1,f1)) = ewp_stmt env memenv (List.rev s1.s_node) letspf in
-        let r2,(lets2,(p2,f2)) = ewp_stmt env memenv (List.rev s2.s_node) letspf in
+        let r1,(lets1,f1) = ewp_stmt env memenv (List.rev s1.s_node) letspf in
+        let r2,(lets2,f2) = ewp_stmt env memenv (List.rev s2.s_node) letspf in
         if List.is_empty r1 && List.is_empty r2 then begin
-          let p1 = mk_let_of_lv_substs env (lets1,p1) in
           let f1 = mk_let_of_lv_substs env (lets1,f1) in
-          let p2 = mk_let_of_lv_substs env (lets2,p2) in
           let f2 = mk_let_of_lv_substs env (lets2,f2) in
           let m = EcMemory.memory memenv in
           let e = form_of_expr m e in
-          let p = f_if e p1 p2 in
           let f = f_if e f1 f2 in
-          ([], (p, f))
+          ([], f)
         end else raise No_wp
 
       | _ -> raise No_wp
@@ -135,20 +130,14 @@ end
 
 let wp ?(uselet=true) ?(onesided=false) ?c_pre env m s post =
   let (r,letsf), cost =
-    LowInternal.wp_stmt
-      onesided c_pre env m (List.rev s.s_node)
-      ([],post) f_x0
-  in
+    LowInternal.wp_stmt onesided c_pre env m (List.rev s.s_node) ([],post) f_x0 in
   let pre = mk_let_of_lv_substs ~uselet env letsf in
   List.rev r, pre, cost
 
-let ewp ?(uselet=true) env m s post epost =
-  let r,(lets,(p,f)) =
-    LowInternal.ewp_stmt env m (List.rev s.s_node) ([],(post, epost))
-  in
-  let pre = mk_let_of_lv_substs ~uselet env (lets,p) in
-  let epre = mk_let_of_lv_substs ~uselet env (lets,f) in
-  (List.rev r, (pre, epre))
+let ewp ?(uselet=true) env m s post =
+  let r,(lets,f) = LowInternal.ewp_stmt env m (List.rev s.s_node) ([],post) in
+  let pre = mk_let_of_lv_substs ~uselet env (lets,f) in
+  (List.rev r, pre)
 
 (* -------------------------------------------------------------------- *)
 module TacInternal = struct
@@ -173,10 +162,10 @@ module TacInternal = struct
     let hs = tc1_as_ehoareS tc in
     let (s_hd, s_wp) = o_split i hs.ehs_s in
     let s_wp = EcModules.stmt s_wp in
-    let (s_wp, (post, epost)) = ewp ~uselet env hs.ehs_m s_wp hs.ehs_po hs.ehs_epo in
+    let (s_wp, post) = ewp ~uselet env hs.ehs_m s_wp hs.ehs_po in
     check_wp_progress tc i hs.ehs_s s_wp;
     let s = EcModules.stmt (s_hd @ s_wp) in
-    let concl = f_eHoareS_r { hs with ehs_s = s; ehs_po = post; ehs_epo = epost} in
+    let concl = f_eHoareS_r { hs with ehs_s = s; ehs_po = post} in
     FApi.xmutate1 tc `Wp [concl]
 
   let t_choare_wp ?(uselet=true) i c_pre tc =
